concurrency/semax_preservation_acquire.v
@@ -645,7 +645,8 @@ Proof.
       -- apply jsafe_phi_age_to; auto. apply jsafe_phi_downward. assumption.
       -- intros c' Ec'; spec safety c' Ec'. apply jsafe_phi_age_to; auto.
          apply jsafe_phi_downward. assumption.
-      -- auto.
+      -- destruct safety as (q_new & Einit & safety). exists q_new; split; auto.
+         apply jsafe_phi_age_to; auto. apply jsafe_phi_downward, safety.
   
   + (* well_formedness *)
     intros j lj.
